Changing Minterop again with a lot of breaking changes

IIO.ML.fst
@@ -1,22 +1,25 @@
-module IO.ML
+module IIO.ML
 
 open FStar.All
 open Common
 open IO.Free
 
+assume val ml_gettrace : args GetTrace -> ML (res GetTrace)
 assume val ml_openfile : args Openfile -> ML (res Openfile)
 assume val ml_read : args Read -> ML (res Read)
 assume val ml_close : args Close -> ML (res Close)
 
-val ml_io_all : (cmd:io_cmds) -> args cmd -> ML (res cmd)
+val ml_io_all : (cmd:cmds) -> args cmd -> ML (res cmd)
 let ml_io_all cmd args =
   match cmd with
+  | GetTrace -> ml_gettrace args
   | Openfile -> ml_openfile args
   | Read -> ml_read args
   | Close -> ml_close args
+  | Throw -> raise args
 
 
-val ml_io_execute : (cmd:io_cmds) -> args cmd -> ML (maybe (res cmd))
+val ml_io_execute : (cmd:cmds) -> args cmd -> ML (resm cmd)
 let ml_io_execute cmd argz =
   try_with
     (fun _ -> Inl (ml_io_all cmd argz))
