Minterop.fst
@@ -1,5 +1,6 @@
 module Minterop
 
+open FStar.All
 open FStar.Tactics
 open FStar.Tactics.Typeclasses
 open Common
@@ -8,6 +9,8 @@ open IO.Effect
 open IIO.Effect
 open MIO.Effect
 open MIIO.Effect
+
+open IIO.ML
 
 (**
 lift: IO -> IIO (Done - in IIO.Effect.fst)
@@ -47,9 +50,7 @@ instance ml_bool : ml bool = { mldummy = () }
 instance ml_int : ml int = { mldummy = () }
 instance ml_string : ml string = { mldummy = () }
 instance ml_pair t1 t2 {| ml t1 |} {| ml t2 |} : ml (t1 * t2) = { mldummy = () }
-instance ml_mioarrow t1 t2 {| ml t1 |} {| ml t2 |} : ml (t1 -> MIO t2) =
-  { mldummy = () }
-instance ml_miioarrow t1 t2 {| ml t1 |} {| ml t2 |} : ml (t1 -> MIIO t2) =
+instance ml_mlarrow t1 t2 {| ml t1 |} {| ml t2 |} : ml (t1 -> ML t2) =
   { mldummy = () }
 
 instance ml_file_descr : ml file_descr = { mldummy = () }
@@ -89,7 +90,7 @@ class importable (t : Type) =
   { itype : Type; import : itype -> option t; ml_itype : ml itype }
 
 class exn_importable (t : Type) =
-  { eitype : Type; exn_import : eitype -> MIO t; ml_eitype : ml eitype }
+  { eitype : Type; exn_import : eitype -> ML t; ml_eitype : ml eitype }
 class safe_importable (t : Type) =
   { sitype : Type; safe_import : sitype -> t; ml_sitype : ml sitype }
 
@@ -104,7 +105,7 @@ let mk_importable
 
 let mk_exn_importable
   (t1 #t2 : Type) {| ml t1 |}
-  (imp : t1 -> MIO t2) :
+  (imp : t1 -> ML t2) :
   Tot (exn_importable t2) =
   { eitype = t1; exn_import = imp; ml_eitype = solve }
 
@@ -133,7 +134,7 @@ instance exn_importable_importable t {| d:importable t |} : exn_importable t =
   mk_exn_importable d.itype (fun (x:d.itype) ->
     (match import x with
     | Some x -> x
-    | None -> IO.Effect.throw Contract_failure) <: MIO t)
+    | None -> FStar.All.raise Contract_failure) <: ML t)
 
 instance exportable_refinement
   t {| d:exportable t |}
@@ -145,6 +146,7 @@ class checkable (#t:Type) (p : t -> Type0) =
   { check : (x:t -> b:bool{b ==> p x}) }
 instance general_is_checkeable t (p : t -> bool) : checkable (fun x -> p x) =
   { check = fun x -> p x }
+
 class checkable2 (#t1 #t2:Type) (p : t1 -> t2 -> Type0) =
   { check2 : (x1:t1 -> x2:t2 -> b:bool{b ==> p x1 x2}) }
 instance general_is_checkable2
@@ -172,8 +174,6 @@ instance importable_refinement
       | Some x -> if check #t #rp x then Some x else None
       | None -> None) <: option (x:t{rp x}))
 
-let test_refinement () : MIO (y:int{y = 5}) = exn_import 5
-
 instance exportable_pair
   t1 t2 {| d1:exportable t1 |} {| d2:exportable t2 |} :
   Tot (exportable (t1 * t2)) =
@@ -198,337 +198,119 @@ instance importable_dpair_refined
                if check2 #t1 #t2 #p x y then Some (| x, y |) else None
        | _ -> None) <: option (x:t1 & y:t2{p x y}))
 
-let test_dpair_refined () : MIO (a:int & b:int{b = a + 1}) = exn_import (10, 11)
-
 // A typed term in an untyped context
 instance exportable_arrow
   t1 t2 {| d1:importable t1 |} {| d2:exportable t2 |} :
   Tot (exportable (t1 -> Tot t2))  =
-  mk_exportable (d1.itype -> MIO d2.etype)
+  mk_exportable (d1.itype -> ML d2.etype)
     (fun (f:(t1 -> t2)) ->
       (fun (x:d1.itype) ->
-        export (f (exn_import x)) <: MIO d2.etype))
+        export (f (exn_import x)) <: ML d2.etype))
 
 instance exportable_mlarrow
   t1 t2 {| d1:importable t1 |} {| d2:exportable t2 |} :
-  Tot (exportable (t1 -> MIO t2)) =
-  mk_exportable (d1.itype -> MIO d2.etype)
-    (fun (f:(t1 -> MIO t2)) ->
-      (fun (x:d1.itype) -> export (f (exn_import x)) <: MIO d2.etype))
-
-// An untyped term in a typed context
-instance importable_mlarrow
-  t1 t2 {| d1:exportable t1 |} {| d2:importable t2 |} :
-  Tot (safe_importable (t1 -> MIO t2)) =
-  mk_safe_importable (d1.etype -> MIO d2.itype)
-    (fun (f:(d1.etype -> MIO d2.itype)) ->
-      (fun (x:t1) -> exn_import (f (export x)) <: MIO t2))
-
-// Example trueish
-let trueish (x:int{x >= 0}) : bool = true
-let trueish' (x:int) : MIO bool = (trueish (exn_import x))
-let trueish'' : int -> MIO bool = export trueish
-
-instance importable_darrow_refined
-  (t1:Type) {| d1:exportable t1 |}
-  (t2:Type) {| d2:importable t2 |}
-  (p:t1->t2->Type0) {| d3:checkable2 p |} :
-  Tot (safe_importable (x:t1 -> MIO (y:t2{p x y}))) =
-  mk_safe_importable (d1.etype -> MIO d2.itype) #(x:t1 -> MIO (y:t2{p x y}))
-    (fun (f:(d1.etype -> MIO d2.itype)) ->
-      (fun (x:t1) ->
-        let y : t2 = exn_import (f (export x)) in
-        if check2 #t1 #t2 #p x y then y
-        else IO.Effect.throw Contract_failure))
-
-// Example incr
-
-let incr (x:int) : int = x + 1
-
-let incr2 : int -> MIO int = export incr
-
-let p x y : bool = (y = x + 1)
-let incr'' (x:int) : MIO (y:int{p x y}) = exn_import (incr x)
-
-// TODO: fix this. see https://github.com/FStarLang/FStar/issues/2128
-val incr' : (x:int) -> MIO (y:int{p x y})
-// let incr' = safe_import incr2
+  Tot (exportable (t1 -> ML t2)) =
+  mk_exportable (d1.itype -> ML d2.etype)
+    (fun (f:(t1 -> ML t2)) ->
+      (fun (x:d1.itype) -> export (f (exn_import x)) <: ML d2.etype))
 
 instance exportable_purearrow_spec
   t1 t2 {| d1:importable t1 |} {| d2:exportable t2 |}
   (pre : t1 -> Type0) {| d3:checkable pre |}
   (post : t1 -> t2 -> Type0) :
   Tot (exportable ((x:t1) -> Pure t2 (pre x) (post x))) =
-  mk_exportable (d1.itype -> MIO d2.etype)
+  mk_exportable (d1.itype -> ML d2.etype)
     (fun (f:(x:t1 -> Pure t2 (pre x) (post x))) ->
       (fun (x:d1.itype) ->
         let x : t1 = exn_import x in
         (if check #t1 #pre x then (
           export (f x)
-        ) else IO.Effect.throw Contract_failure) <: MIO d2.etype))
+        ) else FStar.All.raise Contract_failure) <: ML d2.etype))
 
-let _export_IIO_0
-  (#t1:Type)
-  (#t2:Type)
-  (pi:monitorable_prop)
-  (pre:t1 -> trace -> Type0) {| d3:checkable2 pre |}
-  (post: t1 -> trace -> maybe t2 -> trace -> Type0)
-  (f:(x:t1 -> IIO t2 pi (pre x) (post x)))
-  (x:t1) :
-  IIOwp t2 (fun h p -> forall r lt.
-    ((Inr? r /\ Inr?.v r == Contract_failure /\ lt == []) \/
-    post x h r lt) ==> p r lt) = admit();
-  let h = get_trace () in
-  (** TODO: Can any global property help us remove 'enforced_globally'?
-      The context is instrumented, therefore this should check **)
-  if check2 #t1 #trace #pre x h && enforced_globally pi h then
-    f x
-  else IIO.Effect.throw Contract_failure
+let rec run_iio #t1 (t:iio t1) : ML t1 =
+  match t with
+  | Return (Inl r) -> r
+  | Return (Inr r) -> FStar.All.raise r
+  | Call cmd argz fnc ->
+      run_iio #t1 (fnc (ml_io_execute cmd argz))
 
-let _export_IIO
+let _export_MIIO
   (#t1:Type) {| d1:importable t1 |}
   (#t2:Type) {| d2:exportable t2 |}
-  (pi:monitorable_prop)
-  (pre:t1 -> trace -> Type0) {| d3:checkable2 pre |}
-  (post: t1 -> trace -> maybe t2 -> trace -> Type0)
-  (f:(x:t1 -> IIO t2 pi (pre x) (post x)))
+  (f:t1 -> MIIO t2)
   (x:d1.itype) :
-  MIIO d2.etype =
+  ML d2.etype =
   match import x with
-  | Some x -> export (_export_IIO_0 pi pre post f x)
-  | None -> IIO.Effect.throw Contract_failure
+  | Some x ->
+     let tree : iio t2 = reify (f x) [] (fun _ _ -> True) in
+     let r : t2 = run_iio tree in
+     export r
+  | None -> FStar.All.raise Contract_failure
 
-instance exportable_IIO
+instance exportable_IOwp
   (t1:Type) {| d1:importable t1 |}
   (t2:Type) {| d2:exportable t2 |}
-  (pi:monitorable_prop)
   (pre:t1 -> trace -> Type0) {| d3:checkable2 pre |}
-  (post: t1 -> trace -> maybe t2 -> trace -> Type0) :
-  Tot (exportable (x:t1 -> IIO t2 pi (pre x) (post x))) =
-  mk_exportable
-    (d1.itype -> MIIO d2.etype)
-    (_export_IIO pi pre post)
-
-instance exportable_IO
-  (t1:Type) {| d1:importable t1 |}
-  (t2:Type) {| d2:exportable t2 |}
-  (pi:monitorable_prop)
-  (pre:t1 -> trace -> Type0) {| d3:checkable2 pre |}
-  (post: t1 -> trace -> maybe t2 -> trace -> Type0) :
-  Tot (exportable (x:t1 -> IO t2 pi (pre x) (post x))) =
-  mk_exportable
-    (d1.itype -> MIIO d2.etype)
-    (fun (f:(x:t1 -> IO t2 pi (pre x) (post x))) ->
-      _export_IIO pi pre post f)
-
-let rec _import_pi_IIO
-  (#b:Type)
-  (tree : iio b)
-  (pi:monitorable_prop) :
-  IIO b pi (fun _ -> True) (fun _ _ _ -> True) =
-  match tree with
-  | Return (Inl r) -> r
-  | Return (Inr err) -> IIO.Effect.throw err
-  | Call GetTrace argz fnc ->
-      let h = IIO.Effect.get_trace () in
-      let z' : iio b = fnc (Inl h) in
-      rev_append_rev_append ();
-      _import_pi_IIO z' pi
-  | Call (cmd:io_cmds) argz fnc ->
-      (** TODO: The scope of import is to show that export works correctly,
-          therefore instead of using a written dynamic_cmd, would be correct
-          to use the exported version of static_cmd. **)
-      let rez : res cmd = IIO.Effect.dynamic_cmd pi cmd argz in
-      let rezm : resm cmd = Inl rez in
-      let z' : iio b = fnc rezm in
-      rev_append_rev_append ();
-      _import_pi_IIO z' pi
-
-let _import_pre_pi_IIO
-  (#t1:Type) {| d1:exportable t1 |}
-  (#t2:Type) {| d2:importable t2 |}
-  (pi:monitorable_prop)
-  (pre:t1 -> trace -> Type0) {| checkable2 pre |}
-  (f : d1.etype -> MIIO d2.itype)
-  (x:t1) :
-  IIO t2 pi (pre x) (fun _ _ _ -> True) =
-  rev_append_rev_append ();
-  let x' : d1.etype = export x in
-  let h = get_trace () in
-  (** The pre-condition of MIO is always true so we can pass any
-  post-condition to reify **)
-  let tree : iio d2.itype = (* MIO?.*)reify (f x') h (fun _ _ -> True) in
-  let (r:d2.itype) = _import_pi_IIO tree pi in
-  match import r with
-  | Some a -> a
-  | None -> IIO.Effect.throw #t2 Contract_failure
-
-let extract_local_trace (h:trace) (pi:monitorable_prop) :
-  IIO trace pi
-    (requires (fun h' -> suffix_of h h'))
-    (ensures (fun h' r lt ->
-      lt == [] /\
-      Inl? r /\
-      h' == (apply_changes h (Inl?.v r))))
-  =
-  let h' = get_trace () in
-  suffix_of_length h h';
-  let n : nat = (List.length h') - (List.length h) in
-  let (lt, ht) = List.Tot.Base.splitAt n h' in
-  assume (lt @ ht == h');
-  assume (ht == h);
-  List.Tot.Properties.rev_involutive lt;
-  assert (h' == apply_changes h (List.rev lt));
-  List.rev lt
-
-let check4_implies_post
-  (#t1:Type)
-  (#t2:Type)
-  (x:t1)
-  (h:trace)
-  (r:t2)
-  (post:t1 -> trace -> (m:maybe t2) -> trace -> (r:Type0{Inr? m ==> r}))
-  {| d4:checkable4 post |}
-  (rlt:(maybe trace){Inl? rlt})
-  (lt1:trace)
-  (lt2:trace) :
-  Lemma
-   (requires (
-      ((List.rev lt1 @ List.rev lt2 @ h) == (List.rev (Inl?.v rlt) @ h))
-      /\ check4 #t1 #trace #(maybe t2) #trace #post x h (Inl r) (Inl?.v rlt)
-   ))
-   (ensures (post x h (Inl r) (lt2 @ lt1))) =
-     custom_append_inv_tail #event h rlt lt1 lt2
-
-(** TODO: this is trivial. Quite sad to write it **)
-let explain_post_refinement
-  (#t1:Type)
-  (#t2:Type)
   (post:t1 -> trace -> (m:maybe t2) -> trace -> (r:Type0{Inr? m ==> r})) :
-  Lemma (forall x h lt1 lt2. post x h (Inr Contract_failure) (lt1@lt2)) = ()
+  Tot (exportable (x:t1 ->
+    IOwp t2 (fun h p ->
+      pre x h /\ (forall r lt. post x h r lt ==>  p r lt)))) =
+  mk_exportable
+    (d1.itype -> ML d2.etype)
+    (fun (f:(x:t1 -> IOwp t2 (fun h p ->
+      pre x h /\ (forall r lt. post x h r lt ==>  p r lt)))) ->
+      _export_MIIO (_IIOwp_as_MIIO d3.check2 post f))
 
-(** CA: The body of this function was inlined in _import_IIO but the block
-if-then-else added some extra weird goals which did not make sense,
-therefore a fast fix was extracting the block in a different function. **)
-let enforce_post
-  (#t1:Type) {| d1:exportable t1 |}
-  (#t2:Type) {| d2:importable t2 |}
-  (post:t1 -> trace -> (m:maybe t2) -> trace -> (r:Type0{Inr? m ==> r}))
-  {| d4:checkable4 post |}
-  (x:t1)
-  (h:trace)
-  (r:t2)
-  (lt:trace) :
-  IIOwp t2 (fun _ p ->
-    let b = check4 #t1 #trace #(maybe t2) #trace #post x h (Inl r) lt in
-    (b ==>  p (Inl r) []) /\
-    (~b ==>  p (Inr Contract_failure) [])) =
-  (if check4 #t1 #trace #(maybe t2) #trace #post x h (Inl r) lt
-  then r
-  else IIO.Effect.throw #t2 Contract_failure)
+(** The following are valid, but are not useful **)
+// instance exportable_MIO
+//   (t1:Type) {| d1:importable t1 |}
+//   (t2:Type) {| d2:exportable t2 |}
+//   (pi:monitorable_prop) :
+//   Tot (exportable (t1 -> MIO t2)) =
+//   mk_exportable
+//     (d1.itype -> ML d2.etype)
+//     (fun (f:(x:t1 -> MIO t2)) -> _export_MIIO f)
 
+// instance exportable_MIIO
+//   (t1:Type) {| d1:importable t1 |}
+//   (t2:Type) {| d2:exportable t2 |}
+//   (pi:monitorable_prop) :
+//   Tot (exportable (t1 -> MIIO t2)) =
+//   mk_exportable
+//     (d1.itype -> ML d2.etype)
+//     _export_MIIO
 
-(** TODO: why is the binder `x'3 == []` unusable to rewrite the goal. **)
+// instance exportable_IIOwp
+//   (t1:Type) {| d1:importable t1 |}
+//   (t2:Type) {| d2:exportable t2 |}
+//   (pre:t1 -> trace -> Type0) {| d3:checkable2 pre |}
+//   (post: t1 -> trace -> maybe t2 -> trace -> Type0) :
+//   Tot (exportable (x:t1 ->
+//     IIOwp t2 (fun h p ->
+//       pre x h /\ (forall r lt. post x h r lt ==>  p r lt)))) =
+//   mk_exportable
+//     (d1.itype -> ML d2.etype)
+//     (fun f -> _export_MIIO (_IIOwp_as_MIIO pre post f))
 
-(** The post-condition should allow the computation to fail.
-The computation can fail by itself or because it does not
-respect the contracts. It is not reasonable to assume the
-computation handles by itself all errors, therefore the
-context that imported this function should expect errors. **)
-let _import_IIO
-  (#t1:Type) {| d1:exportable t1 |}
-  (#t2:Type) {| d2:importable t2 |}
-  (pi:monitorable_prop)
-  (pre:t1 -> trace -> Type0) {| d3:checkable2 pre |}
-  (post:t1 -> trace -> (m:maybe t2) -> trace -> (r:Type0{Inr? m ==> r}))
-  {| d4:checkable4 post |}
-  (f : (d1.etype -> MIIO d2.itype))
-  (x:t1) :
-  IIO t2 pi (pre x) (post x) by (
-    ignore (pose_lemma (`(suffix_of_append #event ())));
-    ignore (pose_lemma (`(rev_append_rev_append ())));
-    norm [delta_only [`%pure_null_wp;`%pure_assume_wp;`%pure_bind_wp]];
-    norm [delta_only [`%iio_post;`%apply_changes]];
-    ExtraTactics.blowup ();
-    bump_nth 12;
-    ExtraTactics.branch_on (ExtraTactics.get_binder 22);
-    (* Branch 1: Inl *)
-      ExtraTactics.blowup (); (* splits goal in 3 *)
-      smt (); smt ();
+// instance exportable_IO
+//   (t1:Type) {| d1:importable t1 |}
+//   (t2:Type) {| d2:exportable t2 |}
+//   (pi:monitorable_prop)
+//   (pre:t1 -> trace -> Type0) {| d3:checkable2 pre |}
+//   (post: t1 -> trace -> maybe t2 -> trace -> Type0) :
+//   Tot (exportable (x:t1 -> IO t2 pi (pre x) (post x))) =
+//   mk_exportable
+//     (d1.itype -> ML d2.etype)
+//     (fun (f:(x:t1 -> IO t2 pi (pre x) (post x))) ->
+//       _export_MIIO (_IIO_as_MIIO pi pre post f))
 
-      ExtraTactics.branch_on (ExtraTactics.get_binder 27);
-      (* Branch 1.1: Inl *)
-        ExtraTactics.blowup ();
-        bump_nth 7;
-
-        let wp = ExtraTactics.get_binder 15 in
-        let x3 = ExtraTactics.get_binder 19 in
-        let x5 = ExtraTactics.get_binder 23 in
-        l_to_r [`rev_nil; `List.append_l_nil; `List.append_nil_l];
-        let wp' = ExtraTactics.instantiate_multiple_foralls wp
-          [(`(Inr Contract_failure)); (`((`#x3)@(`#x5)))] in
-        mapply wp'
-  )=
-  let h : trace = get_trace () in
-  let f' = _import_pre_pi_IIO pi pre f in
-  let r : t2 = f' x in
-  let lt : trace = extract_local_trace h pi in
-  Classical.forall_intro_2 (
-    Classical.move_requires_2 (
-      check4_implies_post #t1 #t2 x h r post #d4 (Inl lt)));
-  explain_post_refinement post;
-  enforce_post #t1 #d1 #t2 #d2 post #d4 x h r lt
-
-instance importable_MIO_pi_IIO
-  (t1:Type) {| d1:exportable t1 |}
-  (t2:Type) {| d2:importable t2 |}
-  (pre:t1 -> trace -> Type0) {| d3:checkable2 pre |}
-  (post:t1 -> trace -> (m:maybe t2) -> trace -> (r:Type0{Inr? m ==> r}))
-  {| d4:checkable4 post |} :
-  Tot (safe_importable (pi:monitorable_prop -> x:t1 ->
-                              IIO t2 pi (pre x) (post x))) =
-  mk_safe_importable
-    (d1.etype -> MIO d2.itype)
-    #(pi:monitorable_prop -> x:t1 -> IIO t2 pi (pre x) (post x))
-    (fun (f:(d1.etype -> MIO d2.itype)) ->
-      (fun pi -> _import_IIO pi pre post f))
-
-instance importable_MIO_IIO
-  (t1:Type) {| d1:exportable t1 |}
-  (t2:Type) {| d2:importable t2 |}
-  (pi:monitorable_prop)
-  (pre:t1 -> trace -> Type0) {| d3:checkable2 pre |}
-  (post:t1 -> trace -> (m:maybe t2) -> trace -> (r:Type0{Inr? m ==> r}))
-  {| d4:checkable4 post |} :
-  Tot (safe_importable (x:t1 -> IIO t2 pi (pre x) (post x))) =
-  mk_safe_importable
-    (d1.etype -> MIO d2.itype)
-    #(x:t1 -> IIO t2 pi (pre x) (post x))
-    (_import_IIO pi pre post #d4)
-
-instance importable_MIIO_pi_IIO
-  (t1:Type) {| d1:exportable t1 |}
-  (t2:Type) {| d2:importable t2 |}
-  (pre:t1 -> trace -> Type0) {| d3:checkable2 pre |}
-  (post:t1 -> trace -> (m:maybe t2) -> trace -> (r:Type0{Inr? m ==> r}))
-  {| d4:checkable4 post |} :
-  Tot (safe_importable (pi:monitorable_prop -> x:t1 ->
-                               IIO t2 pi (pre x) (post x))) =
-  mk_safe_importable
-    (d1.etype -> MIIO d2.itype)
-    #(pi:monitorable_prop -> x:t1 -> IIO t2 pi (pre x) (post x))
-    (fun (f:(d1.etype -> MIIO d2.itype)) ->
-        (fun pi -> _import_IIO pi pre post f))
-
-instance importable_MIIO_IIO
-  (t1:Type) {| d1:exportable t1 |}
-  (t2:Type) {| d2:importable t2 |}
-  (pi:monitorable_prop)
-  (pre:t1 -> trace -> Type0) {| d3:checkable2 pre |}
-  (post:t1 -> trace -> (m:maybe t2) -> trace -> (r:Type0{Inr? m ==> r}))
-  {| d4:checkable4 post |} :
-  Tot (safe_importable (x:t1 -> IIO t2 pi (pre x) (post x))) =
-  mk_safe_importable
-    (d1.etype -> MIIO d2.itype)
-    #(x:t1 -> IIO t2 pi (pre x) (post x))
-    (_import_IIO pi pre post #d4)
+// instance exportable_IIO
+//   (t1:Type) {| d1:importable t1 |}
+//   (t2:Type) {| d2:exportable t2 |}
+//   (pi:monitorable_prop)
+//   (pre:t1 -> trace -> Type0) {| d3:checkable2 pre |}
+//   (post: t1 -> trace -> maybe t2 -> trace -> Type0) :
+//   Tot (exportable (x:t1 -> IIO t2 pi (pre x) (post x))) =
+//   mk_exportable
+//     (d1.itype -> ML d2.etype)
+//     (fun f -> _export_MIIO (_IIO_as_MIIO pi pre post f))
