MIIO.Effect.fst
@@ -1,7 +1,39 @@
 module MIIO.Effect
 
+open IO.Free
 open IIO.Effect
 
 effect MIIO
   (a:Type) =
   IIOwp a (fun _ p -> forall res le. p res le)
+
+let _IIOwp_as_MIIO
+  (pre:'a -> trace -> bool)
+  (post:'a -> trace -> (m:maybe 'b) -> trace -> (r:Type0))
+  (f:(x:'a ->
+    IIOwp 'b (fun h p -> pre x h /\ (forall r lt. post x h r lt ==> p r lt))))
+  (x:'a) :
+  MIIO 'b =
+  let h = get_trace () in
+  if pre x h then f x
+  else IIO.Effect.throw Contract_failure
+
+(** this is just a backup. not useful anymore. **)
+// let _IIO_as_MIIO
+//   (#t1:Type)
+//   (#t2:Type)
+//   (pi:monitorable_prop)
+//   (pre:t1 -> trace -> Type0) {| d3:checkable2 pre |}
+//   (post: t1 -> trace -> maybe t2 -> trace -> Type0)
+//   (f:(x:t1 -> IIO t2 pi (pre x) (post x)))
+//   (x:t1) :
+//   MIIO t2 =
+//   // IIOwp t2 (fun h p -> forall r lt.
+//     // ((Inr? r /\ Inr?.v r == Contract_failure /\ lt == []) \/
+//     // post x h r lt) ==> p r lt) = admit();
+//   let h = get_trace () in
+//   (** TODO: Can any global property help us remove 'enforced_globally'?
+//       The context is instrumented, therefore this should check **)
+//   if check2 #t1 #trace #pre x h && enforced_globally pi h then
+//     f x
+//   else IIO.Effect.throw Contract_failure
